paper update

plugins/vdm2isa/src/main/resources/RecursiveVDM.thy
@@ -9,30 +9,50 @@ begin
 section \<open>Introduction\label{sec:Intro}\<close>
 
 text \<open>This paper describes a translation strategy for a variety of recursive definitions from 
-VDM to Isabelle/HOL\<^footnote>\<open>\<^url>\<open>https://github.com/leouk/VDM_Toolkit\<close>\<close>. The strategy takes 
+VDM to Isabelle/HOL. The strategy takes 
 into account the differences in how termination and well-foundedness 
-are represented in both formalisms. It is an extension to a VDM to Isabelle/HOL 
-translation strategy and implementation as a plugin to VDMJ~@{cite Battle09} and 
-extension to VDM-VSCode @{cite AdvancedVSCodePaper}.\<close>
+are represented in both formalisms. 
+
+Beyond overcoming technical practicalities, which we discuss, a major objective is to create
+translation strategy templates. These templates must cover a wide variety of VDM 
+recursive definitions, as well as having their proof obligations being highly automated.
+The result is an extension to a VDM to Isabelle/HOL translation strategy and implementation 
+as a plugin to VDMJ~@{cite Battle09} and extension to VDM-VSCode @{cite AdvancedVSCodePaper}.
+
+Isabelle uses literate programming, where formal specification, proofs and documentation are
+all within the same environment. We omit proofs scripts below; the full VDM and Isabelle sources 
+and proofs can be found at the VDM toolkit repository at
+ \<^verbatim>\<open>./plugins/vdm2isa/src/main/resources/RecursiveVDM.*\<close>\<^footnote>\<open>in~\<^url>\<open>https://github.com/leouk/VDM_Toolkit\<close>\<close>.
+
+In the next section, we present background on VDM and Isabelle recursion and measure relations.
+In Section~\ref{sec:VDMTypes} we briefly discuss VDM basic types translation and their
+consequence for recursion. Next, Section~\ref{sec:Recursion} describes how both VDM
+and Isabelle recursive definitions work and how they differ. Our translation strategy
+is then presented in Section~\ref{sec:Strategy} for basic types, sets, maps, and 
+complex recursive patterns. Finally, we conclude in Section~\ref{sec:Conclusion}. 
+\<close>
 
 (**************************************************************************************************)
 section \<open>Background\label{sec:Background}\<close> 
 
 text \<open>The VDM to Isabelle/HOL translator caters for a wide range of the VDM AST. It copes with all kinds 
-of expressions, a variety patterns, all types, imports and exports, functions and specifications,
+of expressions, a variety of patterns, almost all types, imports and exports, functions and specifications,
 traces, and some of state and operations. Even though not all kinds of VDM patterns are allowed,
 the translator copes with most, and where it does not, a corresponding equivalent is possible. Among the 
-expressions, map comprehension is of note, given its complexity.
+expressions, map comprehension is of note, given its complexity. Details can be found at 
+@{cite NimFull and AdvancedVSCodePaper}.
 
-One particular area we want to extend the translation into is the one over recursively defined functions. 
+One particular area we want to extend translation is over recursively defined functions. 
 VDM requires the user to define a measure function to justify why recursion will terminate. It then generates
 proof obligations to ensure totality and termination. 
 
-Moreover, even though measures over recursive type structures are impossible to define in VDM, yet are 
-easily described in Isabelle. For example, it is not possible to write a measure in VDM for a 
-recursive function over a recursive record defining a linked list, such as \<^verbatim>\<open>R :: v: nat n: R\<close>. 
-This is automatically generated for our representation of VDM records in Isabelle as a datatype.   
-  
+Finally, our translation strategy follows the size-change termination (SCT) proof 
+strategy described in @{cite SCT_POPL and SCNP_POPL}. In particular, its SCP (polynomial) and SCNP (non-polynomial)
+subclass of recursive definitions within the SCT, which permits efficient termination certificate checking. 
+Effectively, if every infinite computation would give rise to an infinitely decreasing value sequence 
+(according to the size-change principle), then no infinite computation is possible. Termination problems in 
+this class have a global ranking function of a certain form, which can be found using SAT solving, hence 
+increasing automation.
 
 \<^bold>\<open>ANYTHING ELSE? Related work?\<close>
 \<close>
@@ -44,27 +64,32 @@ text \<open>Isabelle represents natural numbers (\<^typ>\<open>\<nat>\<close>) a
   where all numbers are projections over such constructions (\<^emph>\<open>e.g.\<close>~@{lemma "3 = (Suc (Suc (Suc 0)))" by simp}).   
   Isabelle integers (\<^typ>\<open>\<int>\<close>) are defined as a quotient type involving two natural numbers. Isabelle quotient types are 
   injections into a constructively defined type. Like with integers, other
-  Isabelle numeric types (\<^emph>\<open>e.g.,\<close>~rationals\<^typ>\<open>\<rat>\<close>, reals \<^typ>\<open>\<real>\<close>, \<^emph>\<open>etc\<close>.) are defined in terms of some
+  Isabelle numeric types (\<^emph>\<open>e.g.,\<close>~rationals \<^typ>\<open>\<rat>\<close>, reals \<^typ>\<open>\<real>\<close>, \<^emph>\<open>etc\<close>.) are defined in terms of some
   involved natural number construction. Type conversions (or coercions) are then defined to allow users to jump
-  between type spaces. Nevertheless, Isabelle has no implicit type widening rule for \<^typ>\<open>\<nat>\<close>; instead, it takes the
-  following convention:~@{lemma[show_types] \<open>(0 - x::\<nat>) = 0\<close> by simp}. For mixutre of \<^typ>\<open>\<int>\<close> and \<^typ>\<open>\<nat>\<close>, explicit user-defined
+  between type spaces. Nevertheless, Isabelle has no implicit type widening rule for \<^typ>\<open>\<nat>\<close>; instead, it takes 
+  conventions like @{lemma[show_types] \<open>(0 - x::\<nat>) = 0\<close> by simp}. For expressions involving 
+a mixutre of \<^typ>\<open>\<int>\<close> and \<^typ>\<open>\<nat>\<close> typed terms, explicit user-defined
   type coercions are needed (\<^emph>\<open>e.g.,\<close>~@{lemma[show_types] \<open>(2::\<nat>) - (3::\<int>) = -1\<close> by simp}).
  
    VDM expressions with basic-typed (\<^emph>\<open>\<^bold>\<open>nat\<close>\<close>, \<^emph>\<open>\<^bold>\<open>int\<close>\<close>) variables have specific type widening rules.
-  For example, even if both variables are \<^emph>\<open>\<^bold>\<open>nat\<close>\<close>, the result might be \<^emph>\<open>\<^bold>\<open>int\<close>\<close>. Therefore, our translation 
+  For example, even if both variables are \<^emph>\<open>\<^bold>\<open>nat\<close>\<close>, the result might be \<^emph>\<open>\<^bold>\<open>int\<close>\<close>. 
+(\<^emph>\<open>e.g.,\<close>~in VDM \<^verbatim>\<open>0 - x:nat = -x:int\<close>). Therefore, our translation 
   strategy considers VDM \<^emph>\<open>\<^bold>\<open>nat\<close>\<close> as the Isabelle type \<^typ>\<open>VDMNat\<close>, which is just a type synonym for \<^typ>\<open>\<int>\<close>. This 
   simplifies the translation process to Isabelle, such that no type coercions are necessary to encode all VDM type widenning rules. 
   On the other hand, this design decision means encoding of recursive functions over \<^emph>\<open>\<^bold>\<open>nat\<close>\<close> to be more complicated 
   than expected, given VDM \<^emph>\<open>\<^bold>\<open>nat\<close>\<close> is represented as Isabelle's \<^typ>\<open>\<int>\<close>.
-\<close>
+
+  Despite this design decision over basic types and their consequences, recursion
+over VDM \<^emph>\<open>\<^bold>\<open>int\<close>\<close>, sets or maps will still be involved. That is because these types 
+are not constructively defined in Isabelle.\<close>
 
 (**************************************************************************************************)
 section \<open>Recursion in VDM and in Isabelle\label{sec:Recursion}\<close>
 
-text \<open>Recursive definitions are pervasive in VDM models. For example, it can be used to perform 
-iterations over numbers, lists, sets, \<^emph>\<open>etc\<close>. An important aspect of every recursive definition
-is an argument that justifies its termination (\<^emph>\<open>i.e.,\<close>~otherwise, the recursion might go on 
-in an infinite loop).
+text \<open>Recursive definitions are pervasive in VDM models. 
+An important aspect of every recursive definition
+is an argument that justifies its termination. Otherwise, the recursion might go on 
+in an infinite loop.
 
 In VDM, this is defined using a recursive measure:~it has the same input type signature as
 the recursive definition, and returns a \<^emph>\<open>\<^bold>\<open>nat\<close>\<close>, which \<^bold>\<open>must\<close> monotonically decrease 
@@ -82,7 +107,7 @@ A simple example of VDM recursive definition is one for calculating the factoria
    measure n;   
 \end{vdmsl} 
 %
-\noindent The VDM recursive measure simply uses \<^verbatim>\<open>n\<close> itself; this works because the only recursive 
+\noindent The VDM recursive measure simply uses the \<^verbatim>\<open>n\<close> input itself. This works because the only recursive 
 call is made with a decreasing value of \<^verbatim>\<open>n\<close>, until it reaches \<^verbatim>\<open>0\<close> and terminates. VDMJ generates 
 three proof obligations for the definition above.
 %
@@ -97,13 +122,21 @@ factorial: subtype obligation at line 6:57
 
 Proof Obligation 3: (Unproved)
 factorial: recursive function obligation at line 5:4
-(forall n:nat & (not (n = 0) => measure_factorial(n) > measure_factorial((n - 1))))
+(forall n:nat & (not (n = 0) => 
+    measure_factorial(n) > measure_factorial((n - 1))))
 \end{vdmsl} 
 %
-\noindent They are trivial to discharge in Isabelle given the definition of \<^verbatim>\<open>measure_factorial\<close> is just \<^verbatim>\<open>n\<close> 
-(\<^emph>\<open>e.g.,\<close>~@{lemma \<open>\<forall> n::\<nat> . \<not> n = 0 \<longrightarrow> n - 1 \<ge> 0\<close> by simp}, @{lemma \<open>\<forall> n::\<nat> . \<not> n = 0 \<longrightarrow> n > n - 1\<close> by simp}).
- 
-In Isabelle, recursive definitions can be provided through primitive recursion or function definitions. 
+\noindent They are trivial to discharge in Isabelle given the measure definition expanded is just 
+@{lemma \<open>\<forall> n::\<nat> . \<not> n = 0 \<longrightarrow> n - 1 \<ge> 0\<close> by simp} and @{lemma \<open>\<forall> n::\<nat> . \<not> n = 0 \<longrightarrow> n > n - 1\<close> by simp}.
+
+Moreover, even though measures over recursive type structures are impossible to define in VDM, they are 
+easily described in Isabelle. For example, it is not possible to write a measure in VDM for a 
+recursive function over a recursive record defining a linked list, such as \<^verbatim>\<open>R :: v: nat n: R\<close>. 
+This is automatically generated for our representation of VDM records in Isabelle as a datatype.
+Other complex recursive patterns are hard/impossible to represent in VDM (see Section~\ref{sec:Complex}).   
+  
+In Isabelle, recursive definitions can be provided through primitive recursion over inputs are 
+constructively defined, or more general function definitions that produces proof obligations. 
 The former insists on definition for each type constructor and only provides simplification rules; whereas
 the latter allow for more sophisticated input patterns and provides simplification, elimination and 
 induction rules, as well as partial function considerations. For the purposes of this paper, we only 
@@ -111,27 +144,31 @@ consider function definitions. Readers can find more about these differences in~
 
 Isabelle recursive functions requires a proof obligation that parameters represent a constructive and 
 compatible pattern, and that recursive calls terminate. Constructive patterns relates to all constructors 
-in data type being defined in the recursion (\<^emph>\<open>e.g.,\<close>~one equation for each of the constructors of \<^typ>\<open>\<nat>\<close>, 
+in data type being used in the recursion inputs (\<^emph>\<open>e.g.,\<close>~one equation for each of the constructors of \<^typ>\<open>\<nat>\<close>, 
 hence one involving \<^term>\<open>0::\<nat>\<close> and another involving \<^term>\<open>Suc n\<close>). Compatible patterns relates to multiple ways 
 patterns can be constructed will boil down to the pattern completeness cases (\<^emph>\<open>e.g.,\<close>~\<^term>\<open>n + 2::\<nat>\<close> being 
-simply multiple calls over defined constructors like \<^term>\<open>Suc (Suc n)\<close>). That is important to ensure that recursion 
+simply multiple calls over defined constructors like \<^term>\<open>Suc (Suc n)\<close>). This is important to ensure that recursion 
 is well structured (\<^emph>\<open>i.e.,\<close>~recursive calls will not get stuck because some constructs are not available). 
-For example, if you miss the \<^term>\<open>0::\<nat>\<close> case, eventually the \<^term>\<open>Suc n\<close> case will reach zero and fail as no patterns for zero exist. 
+For example, if you miss the \<^term>\<open>0::\<nat>\<close> case, eventually the \<^term>\<open>Suc n\<close> case will reach zero and fail, as no patterns for zero exist. 
 The proof obligation for termination establishes that the recursion is well-founded. This has to be proved whenever 
-properties of defined function are meant to be total. 
+properties of the defined function are meant to be total. 
 
-Isabelle function definitions can be given with either \<^term>\<open>fun\<close> or \<^term>\<open>function\<close>. The
+Isabelle function definitions can be given with either \<^term>\<open>fun\<close> or \<^term>\<open>function\<close> syntax. The
 former attempts to automatically prove the pattern constructive and compatible proofs and finds a measure 
-for other termination proof obligations. The latter allows the user to do the proof manually, as well as provide a measure relation.
-This relation must be well-formed, which means have a well-ordered induction principle over a partially ordered relation defined as
+for the termination proof obligation. The latter requires the user to do these proofs manually 
+by providing a measure relation. It is better suited for cases where \<^term>\<open>fun\<close> declarations fail, 
+which usually involve complex or ill-defined recursion. 
+
+The termination relation must be well-formed, which means have a
+well-ordered induction principle over a partially ordered relation defined as
 @{thm[display,show_types] wf_def}\<^footnote>\<open>For 
-details on what that means in Isabelle, see the \<^class>\<open>wellorder\<close> theorem @{thm wf} in theory \<^verbatim>\<open>Wellfounded.thy\<close>\<close>. 
+details on what well-ordered induction means in Isabelle, see the \<^class>\<open>wellorder\<close> theorem @{thm wf} in 
+theory \<^verbatim>\<open>Wellfounded.thy\<close> within Isabelle's distribution.\<close>. 
 For example, an Isabelle definition of factorial that it automatically discovers all three proofs can be given as\<close>
 (*
 find_theorems name:wellorder
 print_locale! wellorder *)
-fun factorial :: \<open>\<nat> \<Rightarrow> \<nat>\<close> where 
-  \<open>factorial n = (if n = 0 then 1 else n * (factorial (n - 1)))\<close> 
+fun factorial :: \<open>\<nat> \<Rightarrow> \<nat>\<close> where \<open>factorial n = (if n = 0 then 1 else n * (factorial (n - 1)))\<close> 
 (*
 fun 
   factorial' :: \<open>\<int> \<Rightarrow> \<int>\<close>
@@ -147,31 +184,41 @@ termination
   sledgehammer
 *)
 
-text \<open>This Isabelle definition is pretty much 1-1 with the VDM definition. Nevertheless, as mentioned above, VDM basic types widening rules 
-necessitated we translate them to \<^typ>\<open>VDMNat\<close>, which is just \<^typ>\<open>\<int>\<close>. Moreover, \<^typ>\<open>\<int>\<close> is defined in terms of a pair of \<^typ>\<open>\<nat>\<close>, 
-hence recursion over \<^typ>\<open>\<int>\<close> will be involved. Thus, VDM recursive functions translation to Isabelle will be involved as well. 
-For example, the same version of \<^term>\<open>factorial\<close> defined for \<^typ>\<open>\<int>\<close> will fail with the error that \<^emph>\<open>Could not find 
-lexicographic termination order\<close>. That is, Isabelle manages to discharge the pattern proofs \<^typ>\<open>\<int>\<close>, but not the termination one. 
+text \<open>This Isabelle definition is pretty much 1-1 with the VDM definition. 
+Nevertheless, as mentioned above, VDM basic types widening rules 
+necessitated we translate them to \<^typ>\<open>VDMNat\<close>, which is just \<^typ>\<open>\<int>\<close>. 
+The same version of \<^term>\<open>factorial\<close> defined for \<^typ>\<open>\<int>\<close> will fail with 
+the error that ``\<^emph>\<open>Could not find lexicographic termination order\<close>''. That is, 
+Isabelle manages to discharge the pattern proofs for \<^typ>\<open>\<int>\<close>, but not the termination one. 
+This is because the user must provide a projection relation from the \<^typ>\<open>\<int>\<close> 
+quotient type back into the constructive type \<^typ>\<open>\<nat>\<close>.
 
-Even if we could avoid this VDM basic types translation technicality, the same problem would occur for VDM recursion over
-non constructive types, such as sets or maps. That is, Isabelle only allow recursion over finite sets, which are not defined 
-constructively but inductively (\<^emph>\<open>e.g.,\<close>~@{term finite}. Similarly, Isabelle maps are defined with specialised HOL functions, 
-again with domains that are not constructively defined. The only easy recursive definition translation from VDM to Isabelle are those
-involving lists, given lists in Isabelle are defined constructively and VDM sequences maps directly to them.      
+Even if we could avoid these VDM basic types translation technicality, 
+the same problem would occur for VDM recursion over non constructive types, 
+such as sets or maps. That is, Isabelle only allow recursion over finite sets, 
+which are not defined constructively but inductively. 
+Similarly, Isabelle maps are defined with specialised HOL functions, 
+again with domains that are not constructively defined. The only easy 
+recursive definition translation from VDM to Isabelle are those
+involving lists, given lists in Isabelle are defined constructively and VDM 
+sequences maps directly to them.      
 
-Therefore, defining recursive functions over non-constructive types entail more involved compatibility and completeness proofs.
-They also usually lead to partial function definitions, given Isabelle cannot tell whether termination is immediately obvious. 
-In VDM, however, recursive functions on sets (as well as map domains) are common, hence the need for the extending the translation strategy.\<close>
+Therefore, defining recursive functions over non-constructive types entail 
+more involved compatibility and completeness proofs.
+They also usually lead to partial function definitions, given Isabelle cannot 
+tell whether termination is immediately obvious. 
+In VDM, however, recursive functions on sets (as well as map domains) are common, 
+hence the need for extending our translation strategy.\<close>
 
 (**************************************************************************************************)
-section \<open>VDM recursion translation strategy\<close>
+section \<open>VDM recursion translation strategy\label{sec:Strategy}\<close>
 
 text \<open>We want to identify a translation strategy that will cater for such issues described above not only 
 for basic types, but also for sets, sequences, maps, \<^emph>\<open>etc\<close>. This is important to ensure that the
 translator will cater for most commonly used VDM recursion definition patterns.   
 
 As mentioned in~@{cite VDMJAnnotations and AdvancedVSCodePaper}, it is possible to define formal annotations 
-(as comments), which VDMJ will process and make available for its plugins. For our general translation
+(as comments), which VDMJ will process and make available for its plugins. For our translation
 strategy, we create a new annotation called \<^verbatim>\<open>@IsaMeasure\<close>. It defines a user-provided well-founded 
 measure relation that will participate in the Isabelle proofs of termination. For example, for the 
 factorial function above, the user would have to write
@@ -183,23 +230,28 @@ factorial function above, the user would have to write
   measure n;
 \end{vdmsl}
 %
-\noindent This measure relation corresponds to the relationship between the recursive call (\<^verbatim>\<open>factorial(n-1)\<close>)
-and its defining equation (\<^verbatim>\<open>factorial(n)\<close>), where the filtering condition determines for which values of \<^verbatim>\<open>n\<close>
-should the relation refer to (\<^emph>\<open>e.g.,\<close>~non-zero values). More interesting measure relation examples are defined in Section~\ref{subsec:Complex}.  
+\noindent This measure relation corresponds to the relationship between the recursive 
+call (\<^verbatim>\<open>factorial(n-1)\<close>) and its defining equation (\<^verbatim>\<open>factorial(n)\<close>), where the 
+filtering condition determines for which values of \<^verbatim>\<open>n\<close>
+should the relation refer to (\<^emph>\<open>e.g.,\<close>~non-zero values). More interesting measure 
+relation examples are defined in Section~\ref{subsec:Complex}.  
 
-During translation, the plugin will typecheck the \<^verbatim>\<open>@IsaMeasure\<close> annotation (\<^emph>\<open>i.e.,\<close>~it is a type correct relation over the function signature).
-Next, it will translate the annotation and some automation lemmas as series of Isabelle definitions to be used during the proof
-of termination of translated VDM recursive functions. If no annotation is provided, following similar principles from Isabelle, 
-the plugin will try to automatically infer what the measure relation should based on the structure of the recursive function definition.
-When this fails, the user is informed. Still, even if measure relation synthesis succeeds, the user still have to appropriately use it 
+During translation, the plugin will typecheck the \<^verbatim>\<open>@IsaMeasure\<close> annotation 
+(\<^emph>\<open>i.e.,\<close>~it is a type correct relation over the function signature).
+Next, it will translate the annotation and some automation lemmas as series of 
+Isabelle definitions to be used during the proof
+of termination of translated VDM recursive functions. If no annotation is provided, 
+following similar principles from Isabelle, then the plugin will try to automatically 
+infer what the measure relation should be based on the structure of the recursive 
+function definition. When this fails, then the user is informed. Still, even if
+ measure-relation synthesis succeeds, the user still have to appropriately use it 
 during Isabelle's termination proof. 
 
-In what follows, we will detail the translation strategy for each relevant VDM type. For details over the overall translation 
-strategy, see examples in the distribution\<^footnote>\<open>\<^url>\<open>https://github.com/leouk/VDM_Toolkit\<close>\<close> and~@{cite NimFull}. That is we impose 
-various implicit VDM checks as explicit predicates. For example, VDM sets are always finite, and type invariants over set elements must
-hold for every element.
-%TODO: or the paper on the translation! 
-\<close>
+In what follows, we will detail the translation strategy for each relevant VDM type. 
+For details over the overall translation strategy, see examples in the 
+distribution\<^footnote>\<open>\<^url>\<open>https://github.com/leouk/VDM_Toolkit\<close>\<close> and~@{cite NimFull}. That 
+is, we impose various implicit VDM checks as explicit predicates. For example, VDM 
+sets are always finite, and type invariants over set elements must hold for every element.\<close>
 
 (*-------------------------------------------------------------------------------------------------*)
 subsection \<open>Recursion over VDM basic types (\<^emph>\<open>\<^bold>\<open>nat\<close>\<close>, \<^emph>\<open>\<^bold>\<open>int\<close>\<close>)\label{subsec:VDMNat}\<close>
@@ -218,41 +270,41 @@ text \<open>Next, we define the factorial function through recursion. When the p
    Otherwise, we define factorial pretty much as in the VDM definition.
 
 The \<^term>\<open>domintros\<close> tag tells Isabelle to generate domain predicates, in case this function is not total. 
-Domain predicates are important to our strategy because of course every VDM function will be undefined, when
+Domain predicates are important to our strategy because every VDM function will be undefined, when
 applied outside its precondition. It also generates domain-predicate sensitive proof rules listed below.\<close>
 function (domintros) vdm_factorial :: \<open>VDMNat \<Rightarrow> VDMNat\<close> where
-  \<open>vdm_factorial n =
-    (if pre_vdm_factorial n then
-      (if n = 0 then 1 else n * (vdm_factorial (n - 1)))
-    else undefined)\<close>
+  \<open>vdm_factorial n = (if pre_vdm_factorial n then
+                        (if n = 0 then 1 else n * (vdm_factorial (n - 1)))
+                      else undefined)\<close>
 
   text \<open>The proof obligations for pattern compatibility and completeness are next.
  They are discharged with the usual Isabelle proof strategy for simple recursive patterns with the @{method pat_completeness} method.
-  In the general (see more complex recursive call cases below in Section~\ref{subsec:Complex}), 
+  In the general case discussed in Section~\ref{subsec:Complex}), 
   the user might have goals to discharge.\<close>
   by (pat_completeness, auto) \<^marker>\<open>tag invisible\<close>
 
-text \<open>Various theorems are made available, such as:
-  \<^item> Case analysis @{thm vdm_factorial.cases}
-  \<^item> Elimination rules (partial) @{thm vdm_factorial.pelims}
-  \<^item> Induction rules (partial) @{thm vdm_factorial.pinduct}
-  \<^item> Simplification rules (partial) @{thm vdm_factorial.psimps}
+text \<open>Various theorems are made available, such as: case analysis; and (partial) rules
+for elimination, induction and simplification.
+%Case analysis @{thm vdm_factorial.cases}
+%Elimination rules (partial) @{thm vdm_factorial.pelims}
+%Induction rules (partial) @{thm vdm_factorial.pinduct}
+%Simplification rules (partial) @{thm vdm_factorial.psimps}
 
-Note the last two are partial, module a domain predicate @{term vdm_factorial_dom},
+Note the last two are partial, module the domain predicate @{term vdm_factorial_dom},
 which represents a well-founded relation that ensures termination. That is, if the user does not want
-(or know how to) to prove termination, such domain predicates will follow every application of the 
+(or knows how) to prove termination, such domain predicates will follow every application of the 
 factorial definition, hence imposing users the requirement that such well-founded relation is still missing.
 
 If/when the termination proof is discharged, these p-rules can be simplified into total rules that 
 do not depend on a domain predicate, given a well-founded relation has been provided. Domain predicates
-will complicate user proofs, and also make proof strategy synthesis harder to figure out.
+will complicate user proofs, and also make proof strategy synthesis harder to automate.
 
 Termination proof is discharged by establishing a well-founded relation associated with 
 the function recursive call(s) with respect to its declaration. In our case, the \<^verbatim>\<open>@IsaMeasure\<close>
-annotation is translated as the Isabelle abbreviation. We also implicitly add the filter that the 
+annotation is translated as an Isabelle abbreviation. We also implicitly add the filter that the 
 function precondition holds:~this is important to ensure the termination proof never reaches the \<^term>\<open>undefined\<close> case.  
 The other filter comes from the negated test in the definition if-statement. More complex definitions will
-have more involved filters (see Section~\ref{subsec:Complex}. 
+have more involved filters. 
 We use abbreviation instead of definition to avoid needing to expand the defined term.\<close>
 
 abbreviation vdm_factorial_wf :: \<open>(VDMNat \<times> VDMNat) set\<close> where
@@ -264,9 +316,8 @@ text \<open>Given \<^term>\<open>vdm_factorial\<close> is a simple (non-mutual, 
   @{term int_ge_less_than}.
 
   The first term is defined in terms of the second, which is a subset of our well-formed relation \<^term>\<open>vdm_factorial_wf\<close>. 
-  Isabelle has proofs about the term's well formedness \<^term>\<open>int_ge_less_than\<close>.
-
-  Thus, making the proof our term being well founded trivial, and easily discovered with proof tools like
+  Isabelle has proofs about the term's well formedness of \<^term>\<open>int_ge_less_than\<close>.
+  Thus, making the proof our term being well-founded trivial, and easily discovered with proof tools like
   @{command sledgehammer}. As part of the translation strategy, we then define (and automatically discover the proof of)
   the following lemma. This follows the strategy described in~@{cite KrausSCNP}. 
     %\url{https://www21.in.tum.de/~krauss/papers/scnp-wst.pdf}.\<close>
@@ -274,28 +325,27 @@ lemma l_vdm_factorial_term_wf: \<open>wf (gen_VDMNat_term vdm_factorial_wf)\<clo
   by (simp add: wf_int_ge_less_than wf_Int1) 
 
 termination \<^marker>\<open>tag invisible\<close>
-  text \<open>Finally, we prove termination using the previously proved lemma using the @{method relation} for @{goals}.
-  This simplifies the goal into well formedness of termination relation and that the precondition implies it,
+  text \<open>Finally, we prove termination using the previously proved lemma using the @{method relation}.
+  This simplifies the goal into well-formedness of termination relation and that the precondition implies it,
   both of which are easily proved with simplification in this case.\<close>
   apply (relation \<open>(gen_VDMNat_term vdm_factorial_wf)\<close>) \<^marker>\<open>tag invisible\<close>
-  text \<open>This transforms the mysterious/abstract domain predicate into two new subgoals @{subgoals[display]}\<close>
+  text \<open>This transforms the abstract domain predicate into two new subgoals as @{subgoals[display]}\<close>
   using l_vdm_factorial_term_wf apply presburger \<^marker>\<open>tag invisible\<close>
   by (simp add: pre_vdm_factorial_defs int_ge_less_than_def) \<^marker>\<open>tag invisible\<close>
 
-text \<open>For this simple example, these goals are proved with @{command sledgehammer}. In general, the user will be
+text \<open>For this simple example, these subgoals are proved with @{command sledgehammer}. In general, the user will be
   have to either find the proof, or deal with domain predicates in proofs involving the recursive call.
-
-  After the termination proof is discharged, Isabelle provides total versions of useful rules as:
-  \<^item> Elimination rules (total) @{thm vdm_factorial.elims}   
-  \<^item> Induction rules (total)  @{thm vdm_factorial.induct}
-  \<^item> Simplification rules (total) @{thm vdm_factorial.simps}
+ After the termination proof is discharged, Isabelle provides versions of rules 
+for elimination, induction and simplification that are total and do not depend on 
+the abstract domain predicate. 
 \<close>
 
-text \<open>To make sure our choice is valid (\<^emph>\<open>e.g.,\<close>~doesn't lead to the empty relation), we ensure
+text \<open>To make sure our choice does not lead to the empty relation, we ensure
   that indeed the termination relation is in fact the same as the well founded predicate by proving the next goal.
   This is something users might want to do, but is not part of the translation strategy. In case the measure relation 
   is empty, the recursive call simplification rules will not be useful anyhow.\<close>
-lemma l_vdm_factorial_term_valid: \<open>(gen_VDMNat_term vdm_factorial_wf) = vdm_factorial_wf\<close>
+lemma l_vdm_factorial_term_valid: 
+  \<open>(gen_VDMNat_term vdm_factorial_wf) = vdm_factorial_wf\<close>
   apply (simp add: pre_vdm_factorial_defs) \<^marker>\<open>tag invisible\<close>
   apply (intro equalityI subsetI)\<^marker>\<open>tag invisible\<close>
    apply (simp_all add: int_ge_less_than_def case_prod_beta)\<^marker>\<open>tag invisible\<close>
@@ -308,20 +358,22 @@ text \<open>Next, we extend the translation strategy for basic types for VDM set
  recursively defined VDM function over sets that sums the set elements as
 %
 \begin{vdmsl}[frame=none,basicstyle=\ttfamily\scriptsize]
-    sumset: set of nat -> nat 
-    sumset(s) == if s = {} then 0 else let e in set s in sumset(s - {e}) + e
-    --@IsaMeasure({(x - { let e in set x in e }, x) | x : set of nat & x <> {}}) 
-    --@Witness(sumset({ 1 }))
-    measure card s;
+  sumset: set of nat -> nat 
+  sumset(s) == if s = {} then 0 else let e in set s in sumset(s - {e}) + e
+  --@IsaMeasure({(x - { let e in set x in e }, x) | x : set of nat & x <> {}}) 
+  --@Witness(sumset({ 1 }))
+  measure card s;
 \end{vdmsl}
 %
 \noindent Like most common VDM recursion over sets, the function consumes the set by picking each 
 set element and them calling the recursive call without the element picked, until the set is empty. 
-The VDM measure states that the recursion is based on the cardinality of the input parameter;~this is 
-not useful for Isabelle's recursive definition proofs and is ignored during translation.
+The VDM measure states that the recursion is based on the cardinality of the input parameter. VDM 
+measures are not suitable for Isabelle proofs, given Isabelle requires a relation;~hence,
+VDM measures are ignored during translation. They might still be useful during proofs as potential 
+witnesses to existentially-quantified goals.
 
-    In Isabelle, the implicit VDM checks are defined as the precondition, which ensures 
-    that the given set contains only natural numbers, and is finite, as defined by \<^term>\<open>inv_VDMSet'\<close>\<close>
+In Isabelle, the implicit VDM checks are defined as the precondition, which ensures 
+that the given set contains only natural numbers, and is finite, as defined by \<^term>\<open>inv_VDMSet'\<close>\<close>
 
 definition pre_sumset :: \<open>VDMNat VDMSet \<Rightarrow> \<bool>\<close> where
   \<open>pre_sumset s \<equiv> inv_VDMSet' inv_VDMNat s\<close>
@@ -330,17 +382,16 @@ lemmas pre_sumset_defs = pre_sumset_def inv_VDMSet'_defs inv_VDMNat_def
 
 text \<open>We define the VDM recursive function in Isabelle next. It checks whether the given
       set satisfy the function precondition, returning \<^term>\<open>undefined\<close> if not.
-      If it does, then each case is encoded pretty much 1-1 from VDM. The translation strategy for
+      Each case is encoded pretty much 1-1 from VDM after that. The translation strategy for
       VDM \<^verbatim>\<open>let-in-set\<close> patterns uses Isabelle's Hilbert's choice operator (\<^term>\<open>\<some> x . x \<in> s\<close>).
     Note this naturally extends to VDM's \<^verbatim>\<open>let-be-st\<close> patterns as well.\<close>
 function (domintros) sumset :: \<open>VDMNat VDMSet \<Rightarrow> VDMNat\<close> where 
   \<open>sumset s = 
     (if pre_sumset s then 
-        (if s = {} then 0 else 
-            let e = (\<some> x . x \<in> s) in sumset (s - {e}) + e) 
+        (if s = {} then 0 else let e = (\<some> x . x \<in> s) in sumset (s - {e}) + e) 
      else undefined)\<close>
   text \<open>The pattern completeness and compatibility goals are discharged with 
-  the usual proof strategy for this using @{method pat_completeness}.
+  the usual proof strategy of @{method pat_completeness}.
         For more general examples, if that fails, @{command sledgehammer} should be used.
        \<close>
   by (pat_completeness, auto) \<^marker>\<open>tag invisible\<close>
@@ -505,7 +556,18 @@ lemma l_sum_elems_wf_valid: \<open>sum_elems_wf \<noteq> {}\<close>
 (*-------------------------------------------------------------------------------------------------*)
 subsection \<open>VDM recursion involving complex measures\label{subsec:Complex}\<close>
 
-text \<open>
+text \<open>The class of recursive examples shown so far have cover a wide range of 
+situations, and have a good level of automation. Nevertheless, the same strategy can
+also be applied for me complex recursive definitions. The cost for the VDM user
+is the need of a more involved \<^verbatim>\<open>@IsaMeasure\<close> definition and the highly likely need for
+extra user-defined lemmas. These lemmas can be defined in VDM itself using 
+the \<^verbatim>\<open>@Lemma\<close> annotation, which will be translated to Isabelle as any other boolean 
+expression would.
+
+To illustrate this, we define in VDM the (in)famous Ackermann 
+function\<^footnote>\<open>\<^url>\<open>https://en.wikipedia.org/wiki/Ackermann_function\<close>\<close>, 
+which is a staple example of complex recursion, as  
+%
 \begin{vdmsl}[frame=none,basicstyle=\ttfamily\scriptsize]
     ack: nat * nat -> nat 
     ack(m,n) == if m = 0 then n+1
@@ -514,11 +576,121 @@ text \<open>
     --@IsaMeasure( pair_less_VDMNat )
     --@Witness( ack(2, 1) )
     measure is not yet specified;
-\end{vdmsl}\<close>
+\end{vdmsl}
+%
+\noindent Note that the VDM measure is not defined, and that the \<^verbatim>\<open>@IsaMeasure\<close>
+uses a construct from Isabelle called \<^term>\<open>pair_less\<close>. It is part of Isabelle's 
+machinery of concrete orders for SCNP problems @{cite KrausSCNP}. 
+It considers recursions over multiple parameters, where some might 
+increase the number of calls (\<^emph>\<open>e.g.\<close>~size-change). We are not aware of a 
+mechanism to define such measures in VDM. 
 
-text \<open>The plugin has examples of a couple other more complicated recursion. These are Nipkow's 
-permutation function~@{cite TermRewriting} and Takeuchi's 
-function\<^footnote>\<open>\<^url>\<open>https://isabelle.in.tum.de/library/HOL/HOL-Examples/Functions.html\<close>\<close>.
+We instantiate \<^term>\<open>pair_less\<close> to \<^typ>\<open>VDMNat\<close>. It is defined as the lexicographic 
+product over the transitive closure of a totally ordered relation between \<^typ>\<open>VDMNat\<close> 
+inputs\<^footnote>\<open>Details of this definition in the \<^verbatim>\<open>VDMToolkit.thy\<close> file within the 
+distribution in~\<^url>\<open>https://github.com/leouk/VDM_Toolkit\<close>.\<close>. 
+
+If VDM measures were over relations, the Ackermann measure could be defined defined in VDM,
+assuming a standard definition of transitive closure\<^footnote>\<open>The \<^verbatim>\<open>vdmlib/Relations.vdmsl\<close> provides 
+such definition in the VDM toolkit distribution.\<close>, as
+%
+\begin{vdmsl}[frame=none,basicstyle=\ttfamily\scriptsize]
+  pair_less_VDMNat: () -> set of ((nat * nat) * (nat * nat))
+  pair_less_VDMNat() == lex_prod[nat, nat](less_than_VDMNat(), less_than_VDMNat());
+  
+  less_than_VDMNat: () -> set of (nat * nat)
+  less_than_VDMNat() == transitive_closure[nat]({ mk_(z', z) | z', z : nat & z' < z });
+  
+  lex_prod[@A,@B]: set of (@A * @A) * set of (@B * @B) -> set of ((@A * @B) * (@A * @B))
+  lex_prod(ra,rb) == 
+      { mk_(mk_(a, b), mk_(a', b')) | a, a': @A, b, b': @B & 
+          mk_(a,a') in set ra or a = a' and mk_(b, b') in set rb };
+\end{vdmsl}
+%
+That is, the lexicographic product of possibilities that are ordered in its parameters. 
+The translation process is the same as above and produces the Isabelle below. \<close>
+
+definition pre_ack :: \<open>VDMNat \<Rightarrow> VDMNat \<Rightarrow> \<bool>\<close> where
+  \<open>pre_ack m n \<equiv> inv_VDMNat m \<and> inv_VDMNat n\<close>
+
+lemmas pre_ack_defs = pre_ack_def inv_VDMNat_def
+
+function (domintros) ack :: \<open>VDMNat \<Rightarrow> VDMNat \<Rightarrow> VDMNat\<close> where
+  \<open>ack m n = (if pre_ack m n then
+                  if m = 0 then n+1
+             else if n = 0 then ack (m-1) 1
+             else               ack (m-1) (ack m (n-1))
+             else               undefined)\<close>
+  by (pat_completeness, auto) \<^marker>\<open>tag invisible\<close>
+
+abbreviation ack_wf :: \<open>((VDMNat \<times> VDMNat) \<times> (VDMNat \<times> VDMNat)) VDMSet\<close> where
+  \<open>ack_wf \<equiv> pair_less_VDMNat\<close>
+
+termination 
+  apply (relation ack_wf)
+  using wf_pair_less_VDMNat apply blast
+    apply (simp add: inv_VDMNat_def l_pair_less_VDMNat_I1 pre_ack_def)
+   apply (simp add: inv_VDMNat_def pre_ack_def)
+  by (simp add: inv_VDMNat_def pair_less_VDMNat_def pre_ack_def)
+
+text \<open>We also show that this version of Ackermann with \<^typ>\<open>VDMNat\<close> is equivalent to
+  the usual Isabelle definition using \<^typ>\<open>\<nat>\<close>. We omit details here, but have proved
+that they are equivalent by induction\<close>
+
+(*<*)
+fun ack' :: \<open>\<nat> \<Rightarrow> \<nat> \<Rightarrow> \<nat>\<close> where
+  "ack' 0 n             = Suc n"
+| "ack' (Suc m) 0       = ack' m 1"
+| "ack' (Suc m) (Suc n) = ack' m (ack' (Suc m) n)"
+
+fun ack'' :: \<open>\<nat> \<Rightarrow> \<nat> \<Rightarrow> \<nat>\<close> where
+  \<open>ack'' m n = (if m = 0 then Suc n else if n = 0 then ack'' (m - 1) 1 else ack'' (m-1) (ack'' m (n -1)))\<close>
+lemma l_ack''_1[simp]: \<open>ack'' 0 n = Suc n\<close> by simp
+lemma l_ack''_2[simp]: \<open>ack'' (Suc m) 0 = ack'' m 1\<close> by simp
+lemma l_ack''_3[simp]: \<open>ack'' (Suc m) (Suc n) = ack'' m (ack'' (Suc m) n)\<close> by simp
+(*>*)
+
+theorem ack_correct: \<open>ack' m n = ack m n\<close>
+  apply (induction \<open>m\<close> \<open>n\<close> rule: ack'.induct) by (simp add: pre_ack_defs)+
+
+text \<open>
+In general, each complex recursion function will require such a setup. Fortunately, 
+Isabelle has a number of options available. Yet, in general, the more complex the recursion, 
+the more users will have to provide further machinery. For example, the next two 
+examples for Nipkow's permutation function~@{cite TermRewriting} and Takeuchi's 
+function\<^footnote>\<open>\<^url>\<open>https://isabelle.in.tum.de/library/HOL/HOL-Examples/Functions.html\<close>\<close> 
+require a rather ellaborate setup (see Appendix~\ref{app:Complex}).\<close>
+
+(**************************************************************************************************)
+section \<open>Discussion and conclusion\label{sec:Conclusion}\<close>
+
+text \<open>In this paper we present a translation strategy from VDM to Isabelle
+for recursive function over basic types, sets and maps. We also present how 
+the strategy works for more complex recursion, such as the Ackermann's function.
+
+The full VDM and Isabelle sources and proofs can be found at the VDM toolkit repository
+at \<^verbatim>\<open>./plugins/vdm2isa/src/main/resources/RecursiveVDM.*\<close>\<^footnote>\<open>\<^url>\<open>https://github.com/leouk/VDM_Toolkit\<close>\<close>.\<close>
+
+paragraph \<open>Future work.~We are implementing the translation strategy in the vdm2isa plugin,
+which should be available for the VDM-VSCode @{cite AdvancedVSCodePaper} extension in the next release.\<close>
+
+(*<*)
+lemma l_sumset_rel_wf': \<open>wf sumset_wf_rel\<close>
+  apply (rule wf_measure[of \<open>\<lambda> s . card s\<close>, THEN wf_subset])\<^marker>\<open>tag invisible\<close>
+  apply (simp add: measure_def inv_image_def less_than_def less_eq)\<^marker>\<open>tag invisible\<close>
+  apply (rule subsetI, simp add: case_prod_beta)\<^marker>\<open>tag invisible\<close>
+  apply (elim exE conjE)\<^marker>\<open>tag invisible\<close>
+  by (metis card_Diff1_less_iff fst_conv inv_Map_defs(2) inv_Map_defs(3) pre_sumset_defs(1) snd_conv some_in_eq)\<^marker>\<open>tag invisible\<close>
+(*>*)
+
+paragraph \<open>Acknowledgements.~We appreciated discussions with Stephan Merz on 
+pointers for complex well-founded recursion proofs in Isabelle, and with Nick
+Battle on limits for VDM recursive measures.\<close>
+
+(**************************************************************************************************)
+section \<open>Further complex examples\label{app:Complex}\<close>
+
+text \<open>
 %
 \begin{vdmsl}[frame=none,basicstyle=\ttfamily\scriptsize]
     perm: int * int * int -> int --nat
@@ -536,23 +708,146 @@ function\<^footnote>\<open>\<^url>\<open>https://isabelle.in.tum.de/library/HOL/
 \noindent The Takeuchi's function is particularly challenging in proofs and the translation strategy 
 stands no chance of finding proofs for such definitions automatically.\<close>
 
-(**************************************************************************************************)
-section \<open>Limitations\<close>
+subsection \<open>Nipkow's permutation function\<close>
 
-(**************************************************************************************************)
-section \<open>Discussion and conclusion\<close>
+definition 
+  pre_perm :: \<open>VDMInt \<Rightarrow> VDMInt \<Rightarrow> VDMInt \<Rightarrow> \<bool>\<close>
+  where
+  \<open>pre_perm m n r \<equiv> 
+      inv_VDMInt m \<and> inv_VDMInt n \<and> inv_VDMInt r \<and> 
+      ((0 < r \<or> 0 < n) \<longrightarrow> m+n+r > 0)\<close>
 
-paragraph \<open>Future work.~\<close>
+lemmas pre_perm_defs = pre_perm_def inv_VDMInt_def inv_True_def
 
-lemma l_sumset_rel_wf': \<open>wf sumset_wf_rel\<close>
-  apply (rule wf_measure[of \<open>\<lambda> s . card s\<close>, THEN wf_subset])\<^marker>\<open>tag invisible\<close>
-  apply (simp add: measure_def inv_image_def less_than_def less_eq)\<^marker>\<open>tag invisible\<close>
-  apply (rule subsetI, simp add: case_prod_beta)\<^marker>\<open>tag invisible\<close>
-  apply (elim exE conjE)\<^marker>\<open>tag invisible\<close>
-  by (metis card_Diff1_less_iff fst_conv inv_Map_defs(2) inv_Map_defs(3) pre_sumset_defs(1) snd_conv some_in_eq)\<^marker>\<open>tag invisible\<close>
+lemma l_pre_perm_trivial[simp]: "(pre_perm m n r) = ((0 < r \<or> 0 < n) \<longrightarrow> m+n+r > 0)"
+  unfolding pre_perm_def inv_VDMInt_def by simp
 
-paragraph \<open>Acknowledgements.~Stephan Merz for pointers for complex well-founded recursion proofs.\<close>
+function (domintros)
+  perm :: \<open>VDMInt \<Rightarrow> VDMInt \<Rightarrow> VDMInt \<Rightarrow> VDMInt\<close>
+  where
+  \<open>perm m n r =
+    (if pre_perm m n r then
+      (     if 0 < r then perm m (r-1) n 
+       else if 0 < n then perm r (n-1) m
+       else m) 
+    else
+      undefined)
+  \<close>
+  by (pat_completeness, auto)
 
+definition 
+  perm_wf_rel :: \<open>((VDMInt \<times> VDMInt \<times> VDMInt) \<times> (VDMInt \<times> VDMInt \<times> VDMInt)) VDMSet\<close>
+  where
+  \<open>perm_wf_rel \<equiv> 
+      ({ ((m, r-1, n), (m, n, r)) | m r n . 0 < r \<and> pre_perm m n r} 
+      \<union>
+      { ((r, n-1, m), (m, n, r)) | m r n . \<not> 0 < r \<and> 0 < n \<and> pre_perm m n r }
+      )    
+  \<close>
+
+lemma l_perm_wf_rel: "wf perm_wf_rel" 
+proof -
+  text \<open>The Isabelle measure projection reflects the VDM measure: the sum of each parameter.
+        ending up at zero (i.e. if negative, ignore).\<close>
+  have "perm_wf_rel \<subseteq> measure (\<lambda> (m, r, n) . nat (max 0 (m+r+n)))"
+    apply (intro subsetI, case_tac x)
+    apply (simp add: perm_wf_rel_def case_prod_beta max_def)
+    apply (elim disjE conjE, simp) 
+     apply (intro impI conjI, simp_all)
+    text \<open>The setup with @{term perm_wf_rel} works here if the @{term pre_perm} 
+      specifically curbs negative sums of parameters. Yet, the termination proof fails. 
+      Tried various variations on gr or geq etc, no luck. Trying the @{term \<open>mlex_prod\<close>} style nest instead.\<close>
+    nitpick
+    done
+  then show ?thesis
+    by (rule wf_subset [OF wf_measure])
+qed
+
+text \<open>With the added precondition on @{term pre_perm} about case when sum has to be positive,
+      and the well founded proof above, the result worked well\<close>
+termination 
+  apply (relation \<open>perm_wf_rel\<close>)
+    apply (simp add: l_perm_wf_rel)
+   apply (simp_all add: perm_wf_rel_def)  
+  done
+
+subsection \<open>Takeuchi's function (from HOL/Examples/Functions.thy)\<close>
+
+function 
+  tak :: "VDMInt \<Rightarrow> VDMInt \<Rightarrow> VDMInt \<Rightarrow> VDMInt" 
+  where
+  "tak x y z = (if x \<le> y then y else tak (tak (x-1) y z) (tak (y-1) z x) (tak (z-1) x y))"
+  by auto
+
+lemma tak_pcorrect:
+  "tak_dom (x, y, z) \<Longrightarrow> tak x y z = (if x \<le> y then y else if y \<le> z then z else x)"
+  thm tak.pinduct tak.psimps
+  apply (induction x y z rule: tak.pinduct) 
+  by (simp add: tak.psimps)
+
+definition tak_m1 where "tak_m1 = (\<lambda>(x,y,z). if x \<le> y then 0 else 1)"
+definition tak_m2 where "tak_m2 = (\<lambda>(x,y,z). nat (Max {x, y, z} - Min {x, y, z}))"
+definition tak_m3 where "tak_m3 = (\<lambda>(x,y,z). nat (x - Min {x, y, z}))"
+
+lemma "(((x1,y1,z1),(x2,y2,z2)) \<in> tak_m3 <*mlex*> {}) \<longleftrightarrow> (nat (x1 - Min {x1, y1, z1}) < nat (x2 - Min {x2, y2, z2}))"
+  apply (simp add: mlex_iff)
+  unfolding tak_m3_def
+  (*apply (simp only: case_prod_beta fst_conv snd_conv) *)
+  by simp
+
+lemma \<open>((x1,y1,z1),(x2,y2,z2)) \<in> (tak_m2 <*mlex*> (tak_m3 <*mlex*> {}))\<close>
+  apply (simp add: mlex_iff)
+  unfolding tak_m3_def tak_m2_def
+  apply (simp only: case_prod_beta fst_conv snd_conv, clarify)
+  oops
+
+lemma l_call1: 
+  \<open>x > y \<Longrightarrow> ((x-1,y,z),(x,y,z)) \<in> tak_m1 <*mlex*> (tak_m2 <*mlex*> (tak_m3 <*mlex*> {}))\<close> 
+  apply (simp add: mlex_iff)
+  unfolding tak_m3_def tak_m2_def tak_m1_def
+  apply (simp add: case_prod_beta)
+  unfolding min_def max_def
+  by (simp_all split:if_splits)
+
+lemma l_call2:
+  \<open>x > y \<Longrightarrow> ((y-1,z,x),(x,y,z)) \<in> tak_m1 <*mlex*> (tak_m2 <*mlex*> (tak_m3 <*mlex*> {}))\<close>
+  apply (simp add: mlex_iff)
+  unfolding tak_m3_def tak_m2_def tak_m1_def
+  apply (simp add: case_prod_beta)
+  unfolding  min_def max_def
+  by simp
+
+lemma l_call3:
+  \<open>x > y \<Longrightarrow> ((z-1,x,y),(x,y,z)) \<in> tak_m1 <*mlex*> (tak_m2 <*mlex*> (tak_m3 <*mlex*> {}))\<close>
+  apply (simp add: mlex_iff)
+  unfolding tak_m3_def tak_m2_def tak_m1_def
+  apply (simp add: case_prod_beta)
+  unfolding  min_def max_def
+  by simp
+
+lemma l_call4:
+  \<open>x >y \<Longrightarrow>  tak_dom (z - 1, x, y) \<Longrightarrow>
+       tak_dom (y - 1, z, x) \<Longrightarrow>
+       tak_dom (x - 1, y, z) \<Longrightarrow>
+       ((tak (x - 1) y z, tak (y - 1) z x, tak (z - 1) x y), x, y, z)
+       \<in> tak_m1 <*mlex*> tak_m2 <*mlex*> tak_m3 <*mlex*> {}\<close>
+  apply (simp add: mlex_iff)
+  apply (simp add: tak_pcorrect)
+  unfolding tak_m3_def tak_m2_def tak_m1_def 
+  apply (simp add: case_prod_beta)
+  unfolding  min_def max_def
+  by simp
+
+termination
+  apply (relation "tak_m1 <*mlex*> tak_m2 <*mlex*> tak_m3 <*mlex*> {}") 
+      apply (simp add: wf_mlex)
+     apply (simp add: l_call1)
+     apply (simp add: l_call2)
+     apply (simp add: l_call3)
+  by (simp add: l_call4)
+
+theorem tak_correct: "tak x y z = (if x \<le> y then y else if y \<le> z then z else x)"
+  by (induction x y z rule: tak.induct) auto
 (*<*)
 end
 (*>*)
